theories/models/utp_cml/utp_cml.thy
@@ -54,6 +54,7 @@ no_notation
 
 no_syntax
   "_n_upred_ifthenelse" :: "n_upred \<Rightarrow> n_upred \<Rightarrow> n_upred \<Rightarrow> n_upred" ("if _ then _ else _")
+  "_n_upred_while"      :: "n_upred \<Rightarrow> n_upred \<Rightarrow> n_upred" ("while _ do _ od")
   "_upred_prefixed"      :: "n_pexpr \<Rightarrow> n_upred \<Rightarrow> n_upred" ("_ -> _")
   "_n_upred_index"         :: "('b \<Rightarrow> 'a upred) \<Rightarrow> 'b \<Rightarrow> n_upred" ("_<_>" 50)
   "_n_upred_PrefixSkipCSP" :: "n_pexpr \<Rightarrow> n_upred" ("@_")
